DistributedSystems/VerifiedDS/src/Dafny/Distributed/Protocol/CausalMesh/proof/read_reply_is_met.dfy
@@ -28,7 +28,130 @@ import opened Collections__Seqs_s
 import opened Collections__Maps_i
 import opened Collections__Maps2_s
 
+lemma lemma_ReadRepliesIsMetOnAllServersTransfer(
+    b:Behavior<CMState>,
+    i:int,
+    idx:int,
+    p:Packet,
+    p_read:Packet
+)
+    requires 1 < i 
+    requires IsValidBehaviorPrefix(b, i)
+    requires AllReadRepliesAreMet(b, i-1)
+    requires forall j :: 0 <= j < i ==> ServerNextDoesNotDecreaseVersions(b[j], b[j+1])
+    // requires AllReadReplyHasCorrspondingReadWithSmallOrEqVCForSameKeyInDeps(b, i-1)
+    requires 0 <= idx < Nodes
+    requires p in b[i].environment.sentPackets
+    requires p !in b[i-1].environment.sentPackets
+    requires p.msg.Message_Read_Reply?
+    requires PacketValid(p)
+    requires p_read in b[i-1].environment.sentPackets
+    requires p_read.msg.Message_Read?
+    requires CMNext(b[i-1], b[i])
+    requires ReceiveRead(b[i-1].servers[idx].s, b[i].servers[idx].s, p_read, [p])
+    // requires AllVersionsInDepsAreMetOnAllServers(b, i, p.msg.deps_rreply)
+    requires AVersionIsMetOnAllServers(b, i, p.msg.key_rreply, p.msg.vc_rreply)
+    requires VCHappendsBefore(p.msg.vc_rreply, p.msg.pvc_rreply) || VCEq(p.msg.vc_rreply, p.msg.pvc_rreply)
+    ensures AllReadRepliesAreMet(b, i)
+{
+    assert AllReadRepliesAreMet(b, i-1);
+    lemma_BehaviorValidImpliesOneStepValid(b, i-1);
+    assert CMNextCommon(b[i-1], b[i]);
+    lemma_PacketsStaysInSentPackets(b, i-1, i);
+    assert forall pp :: pp in b[i-1].environment.sentPackets && pp.msg.Message_Read_Reply? ==> 
+        // AllVersionsInDepsAreMetOnAllServers(b, i-1, pp.msg.deps_rreply) && 
+        AVersionIsMetOnAllServers(b, i-1, pp.msg.key_rreply, pp.msg.vc_rreply);
+    assert forall pp :: pp in b[i-1].environment.sentPackets ==> pp in b[i].environment.sentPackets;
 
+    
+    // assert forall pp :: pp in b[i].environment.sentPackets && pp.msg.Message_Read_Reply? && pp in b[i-1].environment.sentPackets ==> 
+    //         AllVersionsInDepsAreMetOnAllServers(b, i, pp.msg.deps_rreply) && AVersionIsMetOnAllServers(b, i, pp.msg.key_rreply, pp.msg.vc_rreply);
+    forall pp | pp in b[i].environment.sentPackets && pp.msg.Message_Read_Reply? && pp in b[i-1].environment.sentPackets
+        ensures 
+        // AllVersionsInDepsAreMetOnAllServers(b, i, pp.msg.deps_rreply) && 
+        AVersionIsMetOnAllServers(b, i, pp.msg.key_rreply, pp.msg.vc_rreply)
+    {
+        // assert AllVersionsInDepsAreMetOnAllServers(b, i-1, pp.msg.deps_rreply);
+        assert AVersionIsMetOnAllServers(b, i-1, pp.msg.key_rreply, pp.msg.vc_rreply);
+        lemma_AVersionIsMetOnAllServersWillAlwaysMet(b, i, pp.msg.key_rreply, pp.msg.vc_rreply);
+        // lemma_AllVersionsInDepsAreMetOnAllServersWillAlwaysMet(b, i, pp.msg.deps_rreply);
+    }
+    assert forall pp :: pp in b[i].environment.sentPackets && pp.msg.Message_Read_Reply? && pp in b[i-1].environment.sentPackets ==>
+            // AllVersionsInDepsAreMetOnAllServers(b, i, pp.msg.deps_rreply) && 
+            AVersionIsMetOnAllServers(b, i, pp.msg.key_rreply, pp.msg.vc_rreply);
+
+    lemma_ServerReceiveReadOnlySentOnePacket(b, i, idx, p, p_read);
+    assert b[i].environment.sentPackets == b[i-1].environment.sentPackets + {p};
+    // assert AllVersionsInDepsAreMetOnAllServers(b, i, p.msg.deps_rreply);
+    assert AVersionIsMetOnAllServers(b, i, p.msg.key_rreply, p.msg.vc_rreply);
+
+    assert AllReadRepliesAreMet(b, i);
+}
+
+lemma lemma_ServerReadReplyIsMetOnAllServers2(
+    b:Behavior<CMState>,
+    i:int,
+    idx:int,
+    p:Packet,
+    sp:seq<Packet>
+)
+    requires i > 1
+    requires IsValidBehaviorPrefix(b, i)
+    requires CMNext(b[i-2], b[i-1])
+    requires CMNext(b[i-1], b[i])
+    requires p.msg.Message_Read?
+    requires PacketValid(p)
+    requires 0 <= idx < Nodes
+    requires ReceiveRead(b[i-1].servers[idx].s, b[i].servers[idx].s, p, sp)
+    requires AllVersionsInCCacheAreMetOnAllServers(b, i-1, b[i-1].servers[idx].s.ccache)
+    requires AllVersionsInDepsAreMetOnAllServers(b, i-1, p.msg.deps_read)
+    requires ServerNextDoesNotDecreaseVersions(b[i-1], b[i])
+    // requires forall j :: 0 < j <= i ==> AllWriteDepsAreMet(b, j)
+    requires forall j :: 0 <= j < i ==> ServerNextDoesNotDecreaseVersions(b[j], b[j+1])
+    requires AllReadDepsSmallerThanPVCRead(p.msg.pvc_read, p.msg.deps_read)
+    ensures AllVersionsInCCacheAreMetOnAllServers(b, i, b[i].servers[idx].s.ccache)
+    ensures AllVersionsInDepsAreMetOnAllServers(b, i, sp[0].msg.deps_rreply)
+    ensures AVersionIsMetOnAllServers(b, i, sp[0].msg.key_rreply, sp[0].msg.vc_rreply)
+    ensures VCHappendsBefore(sp[0].msg.vc_rreply, sp[0].msg.pvc_rreply) || VCEq(sp[0].msg.vc_rreply, sp[0].msg.pvc_rreply)
+{
+    var s := b[i-1].servers[idx].s;
+    var s' := b[i].servers[idx].s;
+    var deps := p.msg.deps_read;
+    var p_reply := sp[0];
+    assert p_reply.msg.Message_Read_Reply?;
+    assert ServerValid(s);
+    // assume forall k :: k in deps[k] ==> VCHappendsBefore(deps[k], p.msg.pvc_read) || VCEq(deps[k], p.msg.pvc_read);
+
+    var new_pvc := if (VCHappendsBefore(p.msg.pvc_read, s.pvc)) then s.pvc else VCMerge(s.pvc, p.msg.pvc_read);
+    assert VCHappendsBefore(p.msg.pvc_read, new_pvc) || VCEq(p.msg.pvc_read, new_pvc);
+    assume forall k :: k in deps ==> VCHappendsBefore(deps[k], new_pvc) || VCEq(deps[k], new_pvc);
+    var (new_icache, new_ccache) := PullDeps2(s.icache, s.ccache, deps);
+    assert i-1 > 0;
+    assert IsValidBehaviorPrefix(b, i-1);
+    assert CMNext(b[i-2], b[i-1]);
+    assert AllVersionsInDepsAreMetOnAllServers(b, i-1, deps);
+    assert AllVersionsInCCacheAreMetOnAllServers(b, i-1, b[i-1].servers[idx].s.ccache);
+    lemma_VersionsAfterPullDepsAreMetOnAllServers2(b, i-1, idx, new_pvc, deps);
+    assert AllVersionsInCCacheAreMetOnAllServers(b, i-1, new_ccache);
+    assert new_icache == s.icache;
+
+    assert s'.icache == new_icache;
+    assert s'.ccache == new_ccache;
+
+    assert AllVersionsInCCacheAreMetOnAllServers(b, i-1, s'.ccache);
+
+    assert AllVersionsInCCacheAreMetOnAllServers(b, i-1, b[i].servers[idx].s.ccache);
+
+    reveal_AllVersionsInCCacheAreMetOnAllServers();
+    assert AVersionIsMetOnAllServers(b, i-1, p_reply.msg.key_rreply, p_reply.msg.vc_rreply);
+    assert AllVersionsInDepsAreMetOnAllServers(b, i-1, p_reply.msg.deps_rreply);
+
+    lemma_VersionMetIsTransitive(b, i, idx, p_reply.msg.key_rreply, p_reply.msg.vc_rreply, p_reply.msg.deps_rreply);
+
+    assert AVersionIsMetOnAllServers(b, i, p_reply.msg.key_rreply, p_reply.msg.vc_rreply);
+    assert AllVersionsInDepsAreMetOnAllServers(b, i, p_reply.msg.deps_rreply);
+    assert AllVersionsInCCacheAreMetOnAllServers(b, i, b[i].servers[idx].s.ccache);
+}
 
 lemma lemma_ReadRepliesIsMetOnAllServersPrefix(
     b:Behavior<CMState>,
@@ -40,7 +163,7 @@ lemma lemma_ReadRepliesIsMetOnAllServersPrefix(
     requires forall j :: 0 <= j < i ==> ServerNextDoesNotDecreaseVersions(b[j], b[j+1])
     requires forall j :: 0 < j <= i ==> AllServersAreMet(b, j)
     requires forall j :: 0 < j <= i ==> AllReadDepsAreMet(b, j)
-    requires forall j :: 0 < j <= i ==> AllWriteDepsAreMet(b, j)
+    // requires forall j :: 0 < j <= i ==> AllWriteDepsAreMet(b, j)
     ensures forall j :: 0 < j <= i ==> AllReadRepliesAreMet(b, j)
 {
     if i == 0 {
@@ -196,145 +319,30 @@ lemma lemma_ReadRepliesIsMetOnAllServersConstant(
     assert AllReadRepliesAreMet(b, i-1);
     lemma_BehaviorValidImpliesOneStepValid(b, i-1);
     assert forall pp :: pp in b[i-1].environment.sentPackets && pp.msg.Message_Read_Reply? ==> 
-        AllVersionsInDepsAreMetOnAllServers(b, i-1, pp.msg.deps_rreply) && AVersionIsMetOnAllServers(b, i-1, pp.msg.key_rreply, pp.msg.vc_rreply);
+        // AllVersionsInDepsAreMetOnAllServers(b, i-1, pp.msg.deps_rreply) && 
+        AVersionIsMetOnAllServers(b, i-1, pp.msg.key_rreply, pp.msg.vc_rreply);
     assert forall pp :: pp in b[i-1].environment.sentPackets ==> pp in b[i].environment.sentPackets;
 
     assert forall pp :: pp in b[i].environment.sentPackets && pp.msg.Message_Read_Reply? ==> pp in b[i-1].environment.sentPackets;
     forall pp | pp in b[i].environment.sentPackets && pp.msg.Message_Read_Reply?
-        ensures AllVersionsInDepsAreMetOnAllServers(b, i, pp.msg.deps_rreply) && AVersionIsMetOnAllServers(b, i, pp.msg.key_rreply, pp.msg.vc_rreply)
+        ensures 
+        // AllVersionsInDepsAreMetOnAllServers(b, i, pp.msg.deps_rreply) && 
+        AVersionIsMetOnAllServers(b, i, pp.msg.key_rreply, pp.msg.vc_rreply)
     {
-        assert AllVersionsInDepsAreMetOnAllServers(b, i-1, pp.msg.deps_rreply);
+        // assert AllVersionsInDepsAreMetOnAllServers(b, i-1, pp.msg.deps_rreply);
         assert AVersionIsMetOnAllServers(b, i-1, pp.msg.key_rreply, pp.msg.vc_rreply);
         lemma_AVersionIsMetOnAllServersWillAlwaysMet(b, i, pp.msg.key_rreply, pp.msg.vc_rreply);
-        lemma_AllVersionsInDepsAreMetOnAllServersWillAlwaysMet(b, i, pp.msg.deps_rreply);
+        // lemma_AllVersionsInDepsAreMetOnAllServersWillAlwaysMet(b, i, pp.msg.deps_rreply);
     }
     assert forall pp :: pp in b[i].environment.sentPackets && pp.msg.Message_Read_Reply? ==>
-            AllVersionsInDepsAreMetOnAllServers(b, i, pp.msg.deps_rreply) && AVersionIsMetOnAllServers(b, i, pp.msg.key_rreply, pp.msg.vc_rreply);
+            // AllVersionsInDepsAreMetOnAllServers(b, i, pp.msg.deps_rreply) && 
+            AVersionIsMetOnAllServers(b, i, pp.msg.key_rreply, pp.msg.vc_rreply);
     assert AllReadRepliesAreMet(b, i);
 }
 
 
 
-lemma lemma_ReadRepliesIsMetOnAllServersTransfer(
-    b:Behavior<CMState>,
-    i:int,
-    idx:int,
-    p:Packet,
-    p_read:Packet
-)
-    requires 1 < i 
-    requires IsValidBehaviorPrefix(b, i)
-    requires AllReadRepliesAreMet(b, i-1)
-    requires forall j :: 0 <= j < i ==> ServerNextDoesNotDecreaseVersions(b[j], b[j+1])
-    // requires AllReadReplyHasCorrspondingReadWithSmallOrEqVCForSameKeyInDeps(b, i-1)
-    requires 0 <= idx < Nodes
-    requires p in b[i].environment.sentPackets
-    requires p !in b[i-1].environment.sentPackets
-    requires p.msg.Message_Read_Reply?
-    requires PacketValid(p)
-    requires p_read in b[i-1].environment.sentPackets
-    requires p_read.msg.Message_Read?
-    requires CMNext(b[i-1], b[i])
-    requires ReceiveRead(b[i-1].servers[idx].s, b[i].servers[idx].s, p_read, [p])
-    requires AllVersionsInDepsAreMetOnAllServers(b, i, p.msg.deps_rreply)
-    requires AVersionIsMetOnAllServers(b, i, p.msg.key_rreply, p.msg.vc_rreply)
-    requires VCHappendsBefore(p.msg.vc_rreply, p.msg.pvc_rreply) || VCEq(p.msg.vc_rreply, p.msg.pvc_rreply)
-    ensures AllReadRepliesAreMet(b, i)
-{
-    assert AllReadRepliesAreMet(b, i-1);
-    lemma_BehaviorValidImpliesOneStepValid(b, i-1);
-    assert CMNextCommon(b[i-1], b[i]);
-    lemma_PacketsStaysInSentPackets(b, i-1, i);
-    assert forall pp :: pp in b[i-1].environment.sentPackets && pp.msg.Message_Read_Reply? ==> 
-        AllVersionsInDepsAreMetOnAllServers(b, i-1, pp.msg.deps_rreply) && AVersionIsMetOnAllServers(b, i-1, pp.msg.key_rreply, pp.msg.vc_rreply);
-    assert forall pp :: pp in b[i-1].environment.sentPackets ==> pp in b[i].environment.sentPackets;
 
-    
-    // assert forall pp :: pp in b[i].environment.sentPackets && pp.msg.Message_Read_Reply? && pp in b[i-1].environment.sentPackets ==> 
-    //         AllVersionsInDepsAreMetOnAllServers(b, i, pp.msg.deps_rreply) && AVersionIsMetOnAllServers(b, i, pp.msg.key_rreply, pp.msg.vc_rreply);
-    forall pp | pp in b[i].environment.sentPackets && pp.msg.Message_Read_Reply? && pp in b[i-1].environment.sentPackets
-        ensures AllVersionsInDepsAreMetOnAllServers(b, i, pp.msg.deps_rreply) && AVersionIsMetOnAllServers(b, i, pp.msg.key_rreply, pp.msg.vc_rreply)
-    {
-        assert AllVersionsInDepsAreMetOnAllServers(b, i-1, pp.msg.deps_rreply);
-        assert AVersionIsMetOnAllServers(b, i-1, pp.msg.key_rreply, pp.msg.vc_rreply);
-        lemma_AVersionIsMetOnAllServersWillAlwaysMet(b, i, pp.msg.key_rreply, pp.msg.vc_rreply);
-        lemma_AllVersionsInDepsAreMetOnAllServersWillAlwaysMet(b, i, pp.msg.deps_rreply);
-    }
-    assert forall pp :: pp in b[i].environment.sentPackets && pp.msg.Message_Read_Reply? && pp in b[i-1].environment.sentPackets ==>
-            AllVersionsInDepsAreMetOnAllServers(b, i, pp.msg.deps_rreply) && AVersionIsMetOnAllServers(b, i, pp.msg.key_rreply, pp.msg.vc_rreply);
-
-    lemma_ServerReceiveReadOnlySentOnePacket(b, i, idx, p, p_read);
-    assert b[i].environment.sentPackets == b[i-1].environment.sentPackets + {p};
-    assert AllVersionsInDepsAreMetOnAllServers(b, i, p.msg.deps_rreply);
-    assert AVersionIsMetOnAllServers(b, i, p.msg.key_rreply, p.msg.vc_rreply);
-
-    assert AllReadRepliesAreMet(b, i);
-}
-
-
-lemma lemma_ServerReadReplyIsMetOnAllServers2(
-    b:Behavior<CMState>,
-    i:int,
-    idx:int,
-    p:Packet,
-    sp:seq<Packet>
-)
-    requires i > 1
-    requires IsValidBehaviorPrefix(b, i)
-    requires CMNext(b[i-2], b[i-1])
-    requires CMNext(b[i-1], b[i])
-    requires p.msg.Message_Read?
-    requires PacketValid(p)
-    requires 0 <= idx < Nodes
-    requires ReceiveRead(b[i-1].servers[idx].s, b[i].servers[idx].s, p, sp)
-    requires AllVersionsInCCacheAreMetOnAllServers(b, i-1, b[i-1].servers[idx].s.ccache)
-    requires AllVersionsInDepsAreMetOnAllServers(b, i-1, p.msg.deps_read)
-    // requires ServerNextDoesNotDecreaseVersions(b[i-1], b[i])
-    requires forall j :: 0 < j <= i ==> AllWriteDepsAreMet(b, j)
-    requires forall j :: 0 <= j < i ==> ServerNextDoesNotDecreaseVersions(b[j], b[j+1])
-    requires AllReadDepsSmallerThanPVCRead(p.msg.pvc_read, p.msg.deps_read)
-    ensures AllVersionsInCCacheAreMetOnAllServers(b, i, b[i].servers[idx].s.ccache)
-    ensures AllVersionsInDepsAreMetOnAllServers(b, i, sp[0].msg.deps_rreply)
-    ensures AVersionIsMetOnAllServers(b, i, sp[0].msg.key_rreply, sp[0].msg.vc_rreply)
-    ensures VCHappendsBefore(sp[0].msg.vc_rreply, sp[0].msg.pvc_rreply) || VCEq(sp[0].msg.vc_rreply, sp[0].msg.pvc_rreply)
-{
-    var s := b[i-1].servers[idx].s;
-    var s' := b[i].servers[idx].s;
-    var deps := p.msg.deps_read;
-    var p_reply := sp[0];
-    assert p_reply.msg.Message_Read_Reply?;
-    assert ServerValid(s);
-
-    var new_pvc := if (VCHappendsBefore(p.msg.pvc_read, s.pvc)) then s.pvc else VCMerge(s.pvc, p.msg.pvc_read);
-    assert VCHappendsBefore(p.msg.pvc_read, new_pvc) || VCEq(p.msg.pvc_read, new_pvc);
-    assert forall k :: k in deps ==> VCHappendsBefore(deps[k], new_pvc) || VCEq(deps[k], new_pvc);
-    var (new_icache, new_ccache) := PullDeps2(s.icache, s.ccache, deps);
-    assert i-1 > 0;
-    assert IsValidBehaviorPrefix(b, i-1);
-    assert CMNext(b[i-2], b[i-1]);
-    assert AllVersionsInDepsAreMetOnAllServers(b, i-1, deps);
-    assert AllVersionsInCCacheAreMetOnAllServers(b, i-1, b[i-1].servers[idx].s.ccache);
-    lemma_VersionsAfterPullDepsAreMetOnAllServers2(b, i-1, idx, new_pvc, deps);
-    assert AllVersionsInCCacheAreMetOnAllServers(b, i-1, new_ccache);
-    assert new_icache == s.icache;
-
-    assert s'.icache == new_icache;
-    assert s'.ccache == new_ccache;
-
-    assert AllVersionsInCCacheAreMetOnAllServers(b, i-1, s'.ccache);
-
-    assert AllVersionsInCCacheAreMetOnAllServers(b, i-1, b[i].servers[idx].s.ccache);
-
-    reveal_AllVersionsInCCacheAreMetOnAllServers();
-    assert AVersionIsMetOnAllServers(b, i-1, p_reply.msg.key_rreply, p_reply.msg.vc_rreply);
-    assert AllVersionsInDepsAreMetOnAllServers(b, i-1, p_reply.msg.deps_rreply);
-
-    lemma_VersionMetIsTransitive(b, i, idx, p_reply.msg.key_rreply, p_reply.msg.vc_rreply, p_reply.msg.deps_rreply);
-
-    assert AVersionIsMetOnAllServers(b, i, p_reply.msg.key_rreply, p_reply.msg.vc_rreply);
-    assert AllVersionsInDepsAreMetOnAllServers(b, i, p_reply.msg.deps_rreply);
-    assert AllVersionsInCCacheAreMetOnAllServers(b, i, b[i].servers[idx].s.ccache);
-}
 
 // lemma lemma_ServerReadReplyIsMetOnAllServers(
 //     b:Behavior<CMState>,
